Forward_Hoare.thy
@@ -4,6 +4,8 @@ theory Forward_Hoare
     and "do_prf" :: prf_goal % "proof"
     and "program" :: prf_decl % "proof"
     and "invariant" :: prf_decl % "proof"
+    and "hoare" :: prf_decl % "proof"
+    and "range" and "pre" and "post"
 begin
 
 ML_file "forward_hoare.ML"
